src/Ast/Printer.dfy
@@ -1,0 +1,213 @@
+module Printer {
+  import opened Basics
+  import opened Ast
+  import Types
+
+  method Program(b3: Program) {
+    print "// B3 program\n";
+    var types := SetToSeq(b3.types);
+    for i := 0 to |types| {
+      print "\n";
+      TypeDecl(types[i]);
+    }
+    var procedures := SetToSeq(b3.procedures);
+    for i := 0 to |procedures| {
+      print "\n";
+      Procedure(procedures[i]);
+    }
+  }
+
+  method TypeDecl(ty: Types.Type) {
+    print "type ", ty, "\n";
+  }
+
+  method Procedure(proc: Procedure) {
+    print "procedure ", proc.name, "(";
+    var params := proc.parameters;
+    var sep := "";
+    for i := 0 to |params| {
+      var param := params[i];
+      print sep;
+      match param.kind {
+        case InOut => print "inout ";
+        case Out => print "out ";
+        case _ =>
+      }
+      print param.name, ": ", param.typ;
+      sep := ", ";
+    }
+    print ")\n";
+
+    PrintAExprs(IndentAmount, "requires", proc.pre);
+
+    match proc.body
+    case None =>
+    case Some(stmt) => Statement(stmt, 0);
+  }
+
+  method Indent(indent: nat) {
+    for i := 0 to indent {
+      print " ";
+    }
+  }
+
+  const IndentAmount := 2
+
+  method Label(lbl: string) {
+    if lbl != "" {
+      print lbl, ": ";
+    }
+  }
+
+
+  method Statement(stmt: Stmt, indent: nat)
+    decreases stmt
+  {
+    Indent(indent);
+
+    match stmt
+    case VarDecl(v) =>
+      print "var ";
+      VariableDecl(v);
+      print "\n";
+
+    case ValDecl(v, rhs) =>
+      print "val ";
+      VariableDecl(v);
+      print " := ";
+      Expression(rhs);
+      print "\n";
+
+    case Assign(lhs, rhs) =>
+      print lhs, " := ";
+      Expression(rhs);
+      print "\n";
+
+    case Block(lbl, stmts) =>
+      Label(lbl);
+      print "{\n";
+      for i := 0 to |stmts| {
+        Statement(stmts[i], indent + IndentAmount);
+      }
+      Indent(indent);
+      print "}\n";
+
+    case Call(proc, args) =>
+      print proc, "(";
+      var sep := "";
+      for i := 0 to |args| {
+        print sep;
+        CallArgument(args[i]);
+        sep := ", ";
+      }
+      print ");\n";
+
+    case Check(e) =>
+      ExpressionStmt("check", e);
+
+    case Assume(e) =>
+      ExpressionStmt("assume", e);
+
+    case Assert(e) =>
+      ExpressionStmt("assert", e);
+
+    case AForall(v, body) =>
+      print "forall ";
+      VariableDecl(v);
+      print " {\n";
+      Statement(body, indent + IndentAmount);
+      Indent(indent);
+      print "}\n";
+
+    case If(cond, thn, els) =>
+      print "if ";
+      Expression(cond);
+      print " {\n";
+      Statement(thn, indent + IndentAmount);
+      Indent(indent);
+      print "} else {\n";
+      Statement(els, indent + IndentAmount);
+      Indent(indent);
+      print "}\n";
+
+    case IfCase(cases) =>
+      Indent(indent);
+      print "if {\n";
+      for i := 0 to |cases| {
+        var cs := cases[i];
+        Indent(indent + IndentAmount);
+        print "case ";
+        Expression(cs.cond);
+        print " =>\n";
+        Statement(cs.body, indent + IndentAmount + IndentAmount);
+      }
+      print "}\n";
+
+    case Loop(lbl, invariants, body) =>
+      Indent(indent);
+      Label(lbl);
+      if invariants == Nil {
+        print "loop {\n";
+      } else {
+        PrintAExprs(indent + IndentAmount, "invariant", invariants);
+        Indent(indent);
+        print "{\n";
+      }
+      Statement(body, indent);
+
+    case Exit(lbl) =>
+      print "exit ", lbl, "\n";
+
+    case Return =>
+      print "return\n";
+
+    case Probe(e) =>
+      ExpressionStmt("probe", e);
+  }
+
+  method VariableDecl(v: Variable) {
+    match v.kind {
+      case InOut => print "inout ";
+      case Out => print "out ";
+      case _ =>
+    }
+    print v.name, " ", v.typ;
+  }
+
+  method CallArgument(arg: CallArgument) {
+    match arg
+    case ArgExpr(e) => Expression(e);
+    case ArgLValue(name) => print name;
+  }
+
+  method PrintAExprs(indent: nat, prefix: string, aexprs: List<AExpr>)
+    decreases aexprs
+  {
+    var a := aexprs;
+    while a != Nil
+      invariant aexprs nonincreases to a
+      decreases a.Length()
+    {
+      print prefix;
+      match a.head {
+        case AExpr(e) =>
+          print " ";
+          Expression(e);
+        case AAssertion(s) =>
+          print "\n";
+          Statement(s, indent + IndentAmount);
+      }
+      a := a.tail;
+    }
+  }
+
+  method ExpressionStmt(prefix: string, e: Expr) {
+    print prefix, " ";
+    Expression(e);
+    print "\n";
+  }
+
+  method Expression(e: Expr) {
+    print "<expr>";
+  }
+}
