src/Solver/SolverExpr.dfy
@@ -2,7 +2,7 @@ module SolverExpr {
   export
     reveals Var, Var.name
     provides SExpr
-    provides CreateIdExpr, CreateEq, CreateNegation, CreateBigAnd
+    provides CreateTrue, CreateIdExpr, CreateEq, CreateNegation, CreateBigAnd
 
   class Var {
     const name: string
@@ -12,9 +12,25 @@ module SolverExpr {
   }
 
   type SExpr // pun: solver expression
+    = string // TODO
 
+  function CreateTrue(): SExpr
+  { "TRUE" } // TODO
   function CreateIdExpr(x: Var): SExpr
+  { x.name } // TODO
   function CreateEq(e0: SExpr, e1: SExpr): SExpr
+  { "(EQ " + e0 + " " + e1 + ")" } // TODO
   function CreateNegation(e: SExpr): SExpr
+  { "(NOT " + e + ")" } // TODO
   function CreateBigAnd(ee: seq<SExpr>): SExpr
+  {  // TODO
+    if |ee| == 0 then
+      CreateTrue()
+    else if |ee| == 1 then
+      ee[0]
+    else
+       "(AND" + ToList(ee) + ")"
+  }
+  function ToList(ee: seq<SExpr>): SExpr
+  { if |ee| == 0 then "" else " " + ee[0] + ToList(ee[1..]) }
 }
